pcuic/theories/PCUICInversion.v
@@ -291,3 +291,11 @@ Section Inversion.
   Qed.
 
 End Inversion.
+
+Lemma case_inversion_data_cty {cf:checker_flags} {Σ Γ ci p c brs mdecl idecl indices} :
+  case_inversion_data Σ Γ ci p c brs mdecl idecl indices ->
+  Σ ;;; Γ |- c : mkApps (tInd ci (puinst p)) (pparams p ++ indices).
+Proof.
+  now intros [].
+Qed.
+
